examples/low-level/crypto/Crypto.AEAD.Lemmas.Part3.fst
@@ -1,0 +1,158 @@
+(* This module includes several lemmas to work with the 
+   invariants defined in Crypto.AEAD.Invariant *)
+module Crypto.AEAD.Lemmas.Part3
+open FStar.UInt32
+open FStar.Ghost
+open Buffer.Utils
+open FStar.Monotonic.RRef
+
+open Crypto.Indexing
+open Crypto.Symmetric.Bytes
+open Crypto.Plain
+open Flag
+
+open Crypto.Symmetric.PRF
+open Crypto.AEAD.Encoding 
+open Crypto.AEAD.Invariant
+
+module HH = FStar.HyperHeap
+module HS = FStar.HyperStack
+
+module MAC = Crypto.Symmetric.MAC
+module CMA = Crypto.Symmetric.UF1CMA
+
+module Plain = Crypto.Plain
+module Cipher = Crypto.Symmetric.Cipher
+module PRF = Crypto.Symmetric.PRF
+
+open Crypto.AEAD.Lemmas
+open Crypto.AEAD.Lemmas.Part2
+
+assume val to_seq_temp: #a:Type -> b:Buffer.buffer a -> l:UInt32.t{v l <= Buffer.length b} -> ST (Seq.seq a)
+  (requires (fun h -> Buffer.live h b))
+  (ensures  (fun h0 r h1 -> h0 == h1 /\ Buffer.live h1 b /\ r == Buffer.as_seq h1 b))
+
+#reset-options "--z3timeout 400 --initial_fuel 1 --max_fuel 1 --initial_ifuel 0 --max_ifuel 0"
+let rec frame_refines (i:id{safeId i}) (mac_rgn:region) 
+		      (entries:Seq.seq (entry i)) (blocks:Seq.seq (PRF.entry mac_rgn i))
+		      (h:mem) (h':mem)
+   : Lemma (requires refines h i mac_rgn entries blocks /\
+		     HS.modifies_ref mac_rgn TSet.empty h h' /\
+		     HS.live_region h' mac_rgn)
+	   (ensures  refines h' i mac_rgn entries blocks)
+	   (decreases (Seq.length entries))
+   = if Seq.length entries = 0 then 
+       ()
+     else let e = SeqProperties.head entries in
+          let b = num_blocks e in 
+         (let blocks_for_e = Seq.slice blocks 0 (b + 1) in
+       	  let entries_tl = SeqProperties.tail entries in
+          let blocks_tl = Seq.slice blocks (b+1) (Seq.length blocks) in
+	  frame_refines i mac_rgn entries_tl blocks_tl h h';
+	  frame_refines_one_entry h i mac_rgn e blocks_for_e h')
+
+let rec frame_refines' (i:id{safeId i}) (mac_rgn:region) 
+		      (entries:Seq.seq (entry i)) (blocks:Seq.seq (PRF.entry mac_rgn i))
+		      (h:mem) (h':mem)
+   : Lemma (requires refines h i mac_rgn entries blocks /\
+		     HH.modifies_rref mac_rgn TSet.empty (HS h.h) (HS h'.h) /\
+		     HS.live_region h' mac_rgn)
+	   (ensures  refines h' i mac_rgn entries blocks)
+	   (decreases (Seq.length entries))
+   = admit()
+
+let modifies_push_pop (h:HS.mem) (h0:HS.mem) (h5:HS.mem) (r:Set.set HH.rid)
+  : Lemma (requires (HS.fresh_frame h h0 /\
+		     HS.modifies_transitively (Set.union r (Set.singleton (HS h0.tip))) h0 h5))
+          (ensures (HS.poppable h5 /\ HS.modifies_transitively r h (HS.pop h5)))
+  = ()
+
+let frame_myinv_push (#i:id) (#rw:rw) (st:state i rw) (h:mem) (h1:mem)
+   : Lemma (requires (my_inv st h /\ 
+		      HS.fresh_frame h h1))
+	   (ensures (my_inv st h1))
+   = if safeId i
+     then frame_refines' i st.prf.mac_rgn (HS.sel h st.log) (HS.sel h (PRF.itable i st.prf)) h h1
+
+
+#reset-options "--z3timeout 400 --initial_fuel 0 --max_fuel 0 --initial_ifuel 0 --max_ifuel 0"
+val refines_to_inv: (i:id) -> (st:state i Writer) -> (nonce:Cipher.iv (alg i)) ->
+		       (aadlen: UInt32.t {aadlen <=^ aadmax}) ->
+		       (aad: lbuffer (v aadlen)) ->
+		       (len: UInt32.t {len <> 0ul}) ->
+		       (plain:plainBuffer i (v len)) -> 
+		       (cipher:lbuffer (v len + v MAC.taglen)) ->
+    ST unit (requires (fun h1 ->
+		      Buffer.live h1 aad /\ 
+		      Plain.live h1 plain /\ 
+		      Buffer.live h1 cipher /\ (
+		      HS (h1.h) `Map.contains` st.prf.mac_rgn /\
+		      h1 `HS.contains` st.log /\
+		      (safeId i ==> (
+			let mac_rgn = st.prf.mac_rgn in
+      			let entries_0 = HS.sel h1 st.log in 
+			let table_1 = HS.sel h1 (PRF.itable i st.prf) in
+     			let p = Plain.sel_plain h1 len plain in
+			let c_tagged = Buffer.as_seq h1 cipher in
+			let c, tag = SeqProperties.split c_tagged (v len) in
+			let ad = Buffer.as_seq h1 aad in
+  			let entry = Entry nonce ad (v len) p c_tagged in
+			h1 `HS.contains` (itable i st.prf) /\
+			refines h1 i mac_rgn (SeqProperties.snoc entries_0 entry) table_1)))))
+          (ensures (fun h1 _ h2 -> 
+      		      Buffer.live h1 aad /\ 
+		      Plain.live h1 plain /\ 
+		      Buffer.live h1 cipher /\ (
+		      inv h2 st /\
+		      (if safeId i then 
+			let mac_rgn = st.prf.mac_rgn in
+      			let entries_0 = HS.sel h1 st.log in 
+			let table_1 = HS.sel h1 (PRF.itable i st.prf) in
+     			let p = Plain.sel_plain h1 len plain in
+			let c_tagged = Buffer.as_seq h1 cipher in
+			let c, tag = SeqProperties.split c_tagged (v len) in
+			let ad = Buffer.as_seq h1 aad in
+  			let entry = Entry nonce ad (v len) p c_tagged in
+  			HS.modifies (Set.singleton st.log_region) h1 h2 /\
+			HS.modifies_ref st.log_region !{HS.as_ref st.log} h1 h2 /\ 
+			HS.sel h2 st.log == SeqProperties.snoc entries_0 entry
+		      else HS.modifies Set.empty h1 h2))))
+let refines_to_inv i st nonce aadlen aad len plain cipher =
+  if safeId i then
+    let h0 = get () in 
+    let ad = to_seq_temp aad aadlen in
+    let p = Plain.load len plain in 
+    let c_tagged = to_seq_temp cipher len in
+    let entry = Entry nonce ad (v len) p c_tagged in
+    st.log := SeqProperties.snoc !st.log entry;
+    let h1 = get () in 
+    let entries = !st.log in
+    let blocks = !(itable i st.prf) in
+    frame_refines i st.prf.mac_rgn entries blocks h0 h1
+  else ()
+
+let lemma_frame_find_mac (#i:id) (#l:nat) (st:PRF.state i) 
+			 (x:PRF.domain i{ctr_0 i <^ x.ctr}) (b:lbuffer l)
+			 (h0:HS.mem) (h1:HS.mem) 
+    : Lemma (requires (modifies_table_above_x_and_buffer st x b h0 h1))
+	    (ensures (prf i ==> (
+		      let r = PRF.itable i st in
+		      let tab0 = HS.sel h0 r in
+		      let tab1 = HS.sel h1 r in
+		      let x0 = {x with ctr=ctr_0 i} in
+		      find_mac tab0 x0 == find_mac tab1 x0)))
+    = admit()		      
+
+open FStar.Heap
+let modifies_fresh_empty (i:id) (n: Cipher.iv (alg i)) (r:rid) (m:CMA.state (i,n)) 
+			 (h0:mem) (h1:mem) (h2:mem) 
+  : Lemma (requires (HS (h0.h) `Map.contains` r /\
+		     HS.modifies_ref r TSet.empty h0 h1 /\
+		    (mac_log ==> 
+		        (let ref = CMA (as_hsref (ilog m.log)) in
+			 HS.frameOf ref == r /\
+			 HS.modifies_ref r (TSet.singleton (HS.as_aref ref)) h1 h2)) /\
+		    (safeId i ==> ~ (m_contains (CMA (ilog m.log)) h0))))
+          (ensures (safeId i ==> HS.modifies_ref r TSet.empty h0 h2))
+  = ()
+
